tests/pkg/cbv_attr/lakefile.lean
@@ -1,0 +1,5 @@
+import Lake
+open System Lake DSL
+
+package user_attr
+@[default_target] lean_lib CbvAttr
